platform/RecPred.v
@@ -1,0 +1,60 @@
+Require Import AutoSep DepList.
+
+Set Implicit Arguments.
+
+
+Fixpoint memoryOut' ls (m : smem' ls) : IL.mem :=
+  match m with
+    | HNil => fun _ => None
+    | HCons a _ v m' => fun a' => if weq a' a then v else memoryOut' m' a'
+  end.
+
+Definition memoryOut (m : smem) : IL.mem := memoryOut' m.
+
+Definition stateOut (p : settings * smem) (sc : W) : settings * state :=
+  (fst p, {| Regs := fun _ => sc; Mem := memoryOut (snd p) |}).
+
+Notation "##1" := (fun sc => ![ fun x : settings * smem => Lift (Var0 (stateOut x sc)) ])%Sep : Sep_scope.
+Notation "##2" := (fun sc => ![ fun x : settings * smem => Lift (Lift (Var0 (stateOut x sc))) ])%Sep : Sep_scope.
+
+Definition predIn (P : settings * state -> PropX W (settings * state)) (sc : W) : HProp :=
+  fun stn sm => P (stateOut (stn, sm) sc).
+
+Ltac make_Himp := match goal with
+                    | [ |- interp _ (![?P] _ ---> ![?Q] _)%PropX ] =>
+                      let H := fresh in assert (P ===> Q); [ | rewrite sepFormula_eq in *; apply H ]
+                  end.
+
+Notation "'badt' name p 'end'" :=
+  {| FName := name;
+    FPrecondition := (fun s => ![ p s#Rp ] s)%PropX;
+    FBody := Diverge;
+    FVars := nil;
+    FReserved := 0 |}
+  (no associativity, at level 95, name at level 0, p at level 0, only parsing) : SPfuncs_scope.
+
+Lemma memoryIn'_irrel : forall ls m m',
+  List.Forall (fun a => m a = m' a) ls
+  -> memoryIn' m ls = memoryIn' m' ls.
+  induction ls; inversion 1; subst; simpl; intuition.
+  f_equal; auto.
+Qed.
+
+Lemma memoryIn'_memoryOut' : forall ls (m : smem' ls),
+  NoDup ls
+  -> memoryIn' (memoryOut' m) ls = m.
+  induction m; inversion 1; subst; simpl; intuition.
+  f_equal.
+  unfold H.mem_get, ReadByte.
+  destruct (weq x x); tauto.
+  erewrite memoryIn'_irrel.
+  eauto.
+  apply Forall_forall; intros.
+  destruct (weq x0 x).
+  subst x; tauto.
+  auto.
+Qed.
+
+Theorem memoryIn_memoryOut : forall m, memoryIn (memoryOut m) = m.
+  intros; apply memoryIn'_memoryOut'; apply H.NoDup_all_addr.
+Qed.
